kalloc/tactics.v
@@ -7,3 +7,5 @@ Ltac auto_contradict := try discriminate; try contradiction.
 
 Ltac if_tac_auto_contradict :=
   if_tac; auto_contradict.
+
+Definition PGSIZE := 4096.
